fixed breakage, and provided some lemmas

concurrency/Modular/bst_inst.v
@@ -33,24 +33,15 @@ Definition t_struct_tree_t := Tstruct _tree_t noattr.
 
 (* Spec of findnext function *)
 (* FOUND = 0, NOTFOUND = 1, NULLNEXT = 2 (NULLNEXT = NULL || NEXT ) *)
-Check data_at.
-Check data_at Ews (tptr tvoid) (default_val (tptr tvoid)) _.
-Check default_val t_struct_tree_t.
-
 Definition findnext_spec :=
   DECLARE _findNext
   WITH x: Z, p: val, n: val, n_pt : val, tp: val, r : node_info, g: gname, sh: share, gv: globals
   PRE [ tptr tvoid, tptr (tptr tvoid), tint ]
           PROP (writable_share sh(*; is_pointer_or_null pa; is_pointer_or_null pb*) )
           PARAMS (p; n; Vint (Int.repr x)) GLOBALS (gv)
-          SEP ((* data_at sh (t_struct_tree_t) (p, n) b *)
-            node_rep_R r.1.1.1 r.1.2 r.2 g ;
+          SEP (node_rep_R r.1.1.1 r.1.2 r.2 g ;
                field_at sh (t_struct_tree_t) [StructField _t] r.1.1.1 p;
-               data_at sh (tptr t_struct_tree_t) n_pt n
-                       (*  *(EX n'', data_at Ews (tptr t_struct_tree_t) n'' n') *) 
-          (* ;
-               data_at sh t_struct_tree (Vint (Int.repr px), (pv, (pa, pb))) tp *)
-               )
+               data_at sh (tptr t_struct_tree_t) n_pt n)
   POST [ tint ]
   EX (stt: enum), EX (n' next : val),
          PROP (match stt with
@@ -58,7 +49,8 @@ Definition findnext_spec :=
                | NN => (n' = next)
                end)
         LOCAL (temp ret_temp (enums stt))
-        SEP (node_rep_R r.1.1.1 r.1.2 r.2 g * field_at sh (t_struct_tree_t) [StructField _t] r.1.1.1 p *
+        SEP (node_rep_R r.1.1.1 r.1.2 r.2 g *
+               field_at sh (t_struct_tree_t) [StructField _t] r.1.1.1 p *
                 data_at sh (tptr t_struct_tree_t) next n).
 
 
@@ -75,14 +67,9 @@ Proof.
   forward.
   forward_if. (* if (_x < _y) *)
   - (* pn->n = pn->p->t->left *)
-    forward. (* t1 = pn->p *)
-    forward. (* t2 = t1->t *)
-    forward. (* t3 = t2->left *)
-    forward.
-    Exists NN.
-    Exists pa pa.
+    repeat forward.
+    Exists NN pa pa.
     entailer !.
-    simpl.
     Exists ga gb x0 v0 pa pb locka lockb.
     entailer !.
   - forward_if.
@@ -96,74 +83,8 @@ Proof.
     forward.
     Exists F p n_pt.
     entailer !.
-    simpl.
     Exists ga gb x0 v0 pa pb locka lockb.
     entailer !.
 Qed.
 
 
-
-
-(* Spec of findnext function *)
-Definition findnext_spec :=
-  DECLARE _findNext
-  WITH x: Z, v: val, b: val, p: val, n: val, tp: val, 
-       pa: val, pb: val, px: Z, pv: val, sh: share, gv: globals
-  PRE [ tptr tvoid, tptr (tptr tvoid), tint ]
-          PROP (writable_share sh; is_pointer_or_null pa; is_pointer_or_null pb)
-          PARAMS (b; Vint (Int.repr x); v) GLOBALS (gv)
-          SEP (data_at sh (t_struct_tree_t) (p, n) b;
-               field_at sh (t_struct_tree_t) [StructField _t] tp p;
-               data_at sh t_struct_tree (Vint (Int.repr px), (pv, (pa, pb))) tp)
-  POST [ tint ]
-  EX (succ: bool), EX (n' : val),
-         PROP (match succ with
-               | true => ((n' = pa /\ (Z.lt (Int.signed (Int.repr x)) (Int.signed (Int.repr px)))) \/
-                         (n' = pb /\ (Z.lt (Int.signed (Int.repr px)) (Int.signed (Int.repr x)))))
-               | false => (n' = p /\ Int.signed (Int.repr x) = Int.signed (Int.repr px))
-               end)
-        LOCAL (temp ret_temp (Vint (if succ then Int.one else Int.zero)))
-        SEP (match succ with
-             | true =>
-               (data_at sh (t_struct_tree) (p, n') b *
-               field_at sh (t_struct_tree_t) [StructField _t] tp p *
-               data_at sh t_struct_tree (Vint (Int.repr px), (pv, (pa, pb))) tp)
-             | false =>
-               (data_at sh (t_struct_tree) (p, n) b *
-               field_at sh (t_struct_tree_t) [StructField _t] tp p *
-               data_at sh t_struct_tree (Vint (Int.repr px), (pv, (pa, pb))) tp)
-             end).
-
-(*
-#[export] Instance pointer_lock : Ghost := discrete_PCM (val * val * range).
-Definition ghost_info : Type := (key * val)%type.
-
-(* This allows the range to be outdated while the ghost_info may be present or absent. *)
-#[export] Instance node_ghost : Ghost := prod_PCM pointer_lock (exclusive_PCM (option ghost_info)).
-Notation node_info := (@G node_ghost).
-
-Definition in_tree (g: gname) (g1 : gname) (pn: val) (lock: val):=
-      ghost_snap (P := gmap_ghost (K := gname)(A := discrete_PCM (val * val)) )
-        ({[g1 := (pn, lock)]}) g.
-
-Lemma in_tree_duplicate g gin pn lock:
-  in_tree g gin pn lock |-- in_tree g gin pn lock * in_tree g gin pn lock.
-Proof. by rewrite - bi.persistent_sep_dup. Qed.
-
-Class NodeRep : Type := {
-  node_rep_R : val -> range -> option (option ghost_info) -> gname -> mpred
-  }.
-
-
-#[export]Instance my_specific_tree_rep : NodeRep := {
-  node_rep_R := fun tp r g_info g =>
-    EX (ga gb : gname), EX (x : Z), EX (v pa pb : val), EX (locka lockb : val),
-      !!(g_info = Some (Some (x, v)) /\ and (Z.le Int.min_signed x) (Z.le x Int.max_signed) /\
-       is_pointer_or_null pa /\ is_pointer_or_null locka /\
-       is_pointer_or_null pb /\ is_pointer_or_null lockb /\
-          (tc_val (tptr Tvoid) v) /\ key_in_range x r = true) &&
-       data_at Ews t_struct_tree ((Vint (Int.repr x)), (v, (pa, pb))) tp * 
-       malloc_token Ews t_struct_tree tp *
-       in_tree g ga pa locka * in_tree g gb pb lockb
-}.
-*)
